Come posso indovinare $\displaystyle\sum_{i=1}^{n}i=(2^{n+1})$ ?$2 \displaystyle\sum_{i=1}^{n}i=1+2+...+(n-1)+n+n+(n-1)+...+2+1=(n+1)+...+(n+1)=n(n+1)=\frac{n(n+1)}{2}=\displaystyle\sum_{i=1}^{n}i$Come posso indovinare $\displaystyle\sum_{i=1}^{n}i^{2}=(2^{n+1})$ ?
#### Teorema 4.2.1:
Sia $f(x)\in R[x]$; e sia $d=Deg(f)$ allora $\implies$
$$\begin{array}{l}
\exists g(x)\in R[x]&& \text{t.c.}&&\displaystyle\sum_{i=0}^{n}f(i)=g(n) \iff \forall n\in N& \text{e}& Deg(g)\leq d+1
\end{array}$$
###### Dimostrazione
Omessa $\square$

##### Definiamo
$g(n)$ si dice una formula chiusa per $\displaystyle\sum_{i=0}^{n}f(i)$
###### Esempio
Per 4.2.1 $\implies \exists g(x) \in R[x]$ t.c.
$$\begin{array}{l}
Deg(g) \leq 3& e&\displaystyle\sum_{i=0}^{n}i^{2}=g(n)\\
\forall n \in N \implies \exists a,b,c,d \in\textsf{I\kern-0.1ex R} & t.c.
\end{array}$$
$$\displaystyle\sum_{i=0}^{n} i^{2}=an^{3}+bn^{2}+cn+d\quad * \iff \forall n \in N$$
Quindi:
$$ 
\begin{matrix}{}
0=d & (n=0)& in\quad *\\
1=a+b+c+d & (n=1)& in\quad *\\
5=a8+b4+c2+d &(n=2)& in\quad *\\
14=a27+b9+c3+d & (n=3)& in\quad *\\
\end{matrix}
$$
Pertanto:
$$ 
\begin{cases}
a+b+c=1\\
8a+4b+2c=5 &\implies c=1-a-b  &\implies\\
\cong 7a +9b+3c = 14\\
\end{cases}
\begin{cases}
8a+4b+2(1-a-b)=5\\
27a+9b+3(1-a-b) = 14\\
\end{cases}

$$

$$
\begin{cases}
6a+2b=3\\
24a+6b= 11\\
\end{cases}
\implies
\begin{cases}
b=\frac{3-6a}{2}\\
24a+6(\frac{3-6a}{2})= 11\\
\end{cases}
\implies 
6a=2 
\implies
a = \frac{1}{3}
$$
$$
\implies b= \frac{3-2}{2} \implies b=\frac{1}{2}\\
$$
$$
\implies c= 1-\frac{1}{3}-\frac{1}{2} \implies c=\frac{1}{6}\\
$$
Concludendo 
$$
\begin{matrix}
\displaystyle\sum_{i=0}^{n}i^{2}=\frac{n^{3}}{3}+\frac{n^{2}}{2}+\frac{n}{6} & \forall n \in N
\end{matrix}
$$
[[4.3 Somme Non Polinominiali|Prossimo Capitolo]] 